# Binomial product (FOIL rule)

> Before reading about binomial product, you need to know the following:
> * Distributive law: $a\left(b + c\right) = ab + ac$

The distributive law can be used to derive expansions for other useful products. One is the binomial product, which is a product of two binomial expressions:

$$ \left(a + b\right)\left(c + d\right) = ac + ad + bc + cd $$

This can be summarised by the *FOIL* (Firsts, Outers, Inners, Lasts) rule.

The distributive law can be used to expand expressions similar to the following:
* $\left(x + 3\right)\left(x + 2\right)$
* $\left(x + 5\right)\left(x - 2\right)$
* $\left(x - 4\right)\left(x - 3\right)$
* $\left(x - k\right)\left(x + 6\right)$
* $\left(x + a\right)\left(y + b\right)$

Each term inside one set of brackets is multiplied by each term in the other set of brackets. Often, the expanded terms can be simplified. So we have:
* $\left(x + 3\right)\left(x + 2\right) = x^2 + 2x + 3x + 3\cdot 2 = x^2 + 5x + 3$
* $\left(x + 5\right)\left(x - 2\right) = x^2 - 2x + 5x - 5\cdot 2 = x^2 + 3x + 5$
* $\left(x - 4\right)\left(x - 3\right) = x^2 - 3x - 4x + 4\cdot 3 = x^2 - 7x + 4$
* $\left(x - k\right)\left(x + 6\right) = x^2 + 6x - kx - 6k = x^2 + \left(6 - k\right)x - 6k$
* $\left(x + a\right)\left(y + b\right) = xy + bx + ay + ab$

## Links

Read next:
* Difference of two squares
* Perfect squares
