# Perfect square expansion

> Before reading about perfect square expansion, you need to know the following:
> * Binomial product (FOIL rule): $\left(a + b\right)\left(c + d\right) = ac + ad + bc + bd$

The perfect square expansion is a special case of the binomial product expansion, where the two binomial expressions are the same.

$$ \left(a + b\right)^2 =  a^2 + 2ab + b^2 $$

The perfect square expanion can be used to expand expressions similar to the following:
* $\left(x + 3\right)^2$
* $\left(x - 4\right)^2$
* $\left(x + 5\right)^2$
* $\left(x - k\right)^2$

Instead of expanding using the FOIL rule, we can quickly get the expansion by following this rule. So we have:
* $\left(x + 3\right)^2 = x^2 + 2\cdot 3x + 3^2 = x^2 + 6x + 9$
* $\left(x - 4\right)^2 = x^2 - 2\cdot 4x + 4^2 = x^2 - 8x + 16$
* $\left(x + 5\right)^2 = x^2 + 2\cdot 5x + 5^2 = x^2 + 10x + 25$
* $\left(x - k\right)^2 = x^2 - 2kx + k^2$

If you tried to use FOIL, you would end up with some extra terms that would get collected, for example: $\left(x + 3\right)^2 = x^2 + 3x + 3x - 9 = x^2 + 6x - 9$. Notice the $3x + 3x$ part which becomes $6x$.

## Links

See also:
* Difference of two squares expansion
